prove c_replace_oracle_evp_aux_aux

Computability/Constructions.lean
@@ -1038,6 +1038,252 @@ end div2
 
 
 
+section replace_oracle
+namespace Nat.RecursiveIn.Code
+def encodeCode_replace_oracle (o:ℕ) : Code → ℕ
+| Code.zero        => 0
+| Code.succ        => 1
+| Code.left        => 2
+| Code.right       => 3
+| Code.oracle      => o
+| Code.pair cf cg  => 2*(2*(Nat.pair (encodeCode cf) (encodeCode cg))  )   + 5
+| Code.comp cf cg  => 2*(2*(Nat.pair (encodeCode cf) (encodeCode cg))  )+1 + 5
+| Code.prec cf cg  => 2*(2*(Nat.pair (encodeCode cf) (encodeCode cg))+1)   + 5
+| Code.rfind' cf   => 2*(2*(encodeCode cf                            )+1)+1 + 5
+def replace_oracle (o:ℕ) := fun n => (encodeCode_replace_oracle o (decodeCode n))
+
+
+
+
+/-- `eval c_replace_oracle (o,code)` = `code` but with calls to oracle replaced with calls to code `o` -/
+def c_replace_oracle_aux :=
+  let o               := left
+  let input_to_decode := succ.comp (left.comp right)
+  let comp_hist       := right.comp right
+  let n               := c_sub.comp₂ input_to_decode (c_const 5)
+  let m               := c_div2.comp $ c_div2.comp n
+  let ml              := c_l_get.comp₂ comp_hist (left.comp m)
+  let mr              := c_l_get.comp₂ comp_hist (right.comp m)
+  let nMod4           := c_mod.comp₂ n (c_const 4)
+  let pair_code       := c_add.comp₂ (            c_mul2.comp $             c_mul2.comp (pair ml mr)) (c_const 5)
+  let comp_code       := c_add.comp₂ (succ.comp $ c_mul2.comp $             c_mul2.comp (pair ml mr)) (c_const 5)
+  let prec_code       := c_add.comp₂ (            c_mul2.comp $ succ.comp $ c_mul2.comp (pair ml mr)) (c_const 5)
+  let rfind'_code     := c_add.comp₂ (succ.comp $ c_mul2.comp $ succ.comp $ c_mul2.comp ml          ) (c_const 5)
+
+  -- c_l_get_last.comp $
+  c_cov_rec
+
+  (c_const 0) $
+
+  c_if_eq_te.comp₄ input_to_decode (c_const 1) (c_const 1) $
+  c_if_eq_te.comp₄ input_to_decode (c_const 2) (c_const 2) $
+  c_if_eq_te.comp₄ input_to_decode (c_const 3) (c_const 3) $
+  c_if_eq_te.comp₄ input_to_decode (c_const 4) o           $
+  c_if_eq_te.comp₄ nMod4           (c_const 0) (pair_code) $
+  c_if_eq_te.comp₄ nMod4           (c_const 1) (comp_code) $
+  c_if_eq_te.comp₄ nMod4           (c_const 2) (prec_code) $
+                                                rfind'_code
+
+-- @[simp] theorem c_replace_oracle_ev_pr:code_prim (c_replace_oracle) := by unfold c_replace_oracle; repeat (constructor; try simp)
+
+@[simp] theorem c_replace_oracle_evp_aux_aux (h:n%4=0):
+Nat.list_get_last (eval_prim O (c_replace_oracle_aux) (Nat.pair o ((n+4)+1)))
+  =
+  -- let m:=n.div2.div2
+  let m:=(n/2)/2
+  let ml := Nat.list_get_last (eval_prim O (c_replace_oracle_aux) (Nat.pair o m.l))
+  let mr := Nat.list_get_last (eval_prim O (c_replace_oracle_aux) (Nat.pair o m.r))
+
+  2*(2*(Nat.pair (ml) (mr))  )   + 5
+  -- if n%4=0 then 2*(2*(Nat.pair (ml) (mr))  )   + 5 else
+  -- if n%4=1 then 2*(2*(Nat.pair (ml) (mr))  )+1 + 5 else
+  -- if n%4=2 then 2*(2*(Nat.pair (ml) (mr))+1)   + 5 else
+  --               2*(2*(ml                )+1)+1 + 5
+
+
+
+ := by
+  -- rw [ml]
+  rw (config := {occs := .pos [1]}) [c_replace_oracle_aux]
+  -- rw [c_replace_oracle_aux]
+  simp only [c_cov_rec_evp_3]
+
+  rw [←c_replace_oracle_aux] -- the key step to simplification. otherwise expression blows up
+
+  simp [eval_prim, h]
+
+  have h3 : (n/2/2).l≤n+4 := by exact le_add_right_of_le (Nat.le_trans (unpair_left_le (n/2/2)) (le_trans (Nat.div_le_self _ _) (Nat.div_le_self _ _)))
+  have h4 : (n/2/2).r≤n+4 := by exact le_add_right_of_le (Nat.le_trans (unpair_right_le (n/2/2)) (le_trans (Nat.div_le_self _ _) (Nat.div_le_self _ _)))
+    
+  unfold c_replace_oracle_aux
+  rw [c_cov_rec_evp_2 h3]
+  rw [c_cov_rec_evp_2 h4]
+
+  simp only [] -- remove local defns
+  simp only [l, r]
+
+  rw [mul_comm]
+  simp? says simp only [mul_eq_mul_left_iff, OfNat.ofNat_ne_zero, or_false]
+  rw [mul_comm]
+
+
+set_option maxHeartbeats 3 in
+@[simp] theorem c_replace_oracle_evp_aux: eval_prim O (c_replace_oracle) (Nat.pair o n) =
+  let m:=n.div2.div2
+  let ml := eval_prim O (c_replace_oracle) (Nat.pair o m.l)
+  let mr := eval_prim O (c_replace_oracle) (Nat.pair o m.r)
+
+  if n=0 then 0 else
+  if n=1 then 1 else
+  if n=2 then 2 else
+  if n=3 then 3 else
+  if n=4 then o else
+  if n%4=0 then 2*(2*(Nat.pair (ml) (mr))  )   + 5 else
+  if n%4=1 then 2*(2*(Nat.pair (ml) (mr))  )+1 + 5 else
+  if n%4=2 then 2*(2*(Nat.pair (ml) (mr))+1)   + 5 else
+                2*(2*(ml                )+1)+1 + 5
+
+
+
+ :=
+ match n with
+  | 0 => by
+    rw [c_replace_oracle]
+    simp [eval_prim]
+  | 1 => by
+    rw [c_replace_oracle]
+    simp [eval_prim]
+  | 2 => by
+    rw [c_replace_oracle]
+    simp [eval_prim]
+  | 3 => by
+    rw [c_replace_oracle]
+    simp [eval_prim]
+  | 4 => by
+    rw [c_replace_oracle]
+    simp [eval_prim]
+  | n + 5 => by
+    sorry
+    -- rw [c_replace_oracle]
+    -- simp [eval_prim]
+--  by
+
+--   rw (config := {occs := .pos [1]}) [c_replace_oracle]
+--   simp [eval_prim]
+--   rw (config := {occs := .pos [1]}) [c_replace_oracle]
+--   simp [eval_prim]
+
+-- set_option maxHeartbeats 1000000 in
+set_option maxHeartbeats 3 in
+@[simp] theorem c_replace_oracle_evp_1: eval_prim O (c_replace_oracle) = unpaired replace_oracle := by
+  sorry
+  funext oc
+  let o:=oc.l
+  let c:=oc.r
+  have oc_eq : oc = Nat.pair o c := by exact Eq.symm (pair_unpair oc)
+  rw [oc_eq]
+
+
+
+  induction c using Nat.strong_induction_on with
+  | _ c ih =>
+    match c with
+    | 0 =>
+      sorry
+      unfold c_replace_oracle
+      unfold replace_oracle
+      simp [encodeCode_replace_oracle, decodeCode]
+      simp [eval_prim]
+    | 1 =>
+      sorry
+      unfold c_replace_oracle
+      unfold replace_oracle
+      simp [encodeCode_replace_oracle, decodeCode]
+      simp [eval_prim]
+    | 2 =>
+      sorry
+      unfold c_replace_oracle
+      unfold replace_oracle
+      simp [encodeCode_replace_oracle, decodeCode]
+      simp [eval_prim]
+    | 3 =>
+      sorry
+      unfold c_replace_oracle
+      unfold replace_oracle
+      simp [encodeCode_replace_oracle, decodeCode]
+      simp [eval_prim]
+    | 4 =>
+      sorry
+      unfold c_replace_oracle
+      unfold replace_oracle
+      simp [encodeCode_replace_oracle, decodeCode]
+      simp [eval_prim]
+    | n + 5 =>
+      let m := n.div2.div2
+      have hm : m < n + 5 := by
+        simp only [m, Nat.div2_val]
+        exact lt_of_le_of_lt (le_trans (Nat.div_le_self _ _) (Nat.div_le_self _ _)) (Nat.succ_le_succ (Nat.le_add_right _ _))
+      have _m1 : m.unpair.1 < n + 5 := lt_of_le_of_lt m.unpair_left_le hm
+      have _m2 : m.unpair.2 < n + 5 := lt_of_le_of_lt m.unpair_right_le hm
+      -- have IH := encodeCode_decodeCode m
+      -- have IH1 := encodeCode_decodeCode m.unpair.1
+      -- have IH2 := encodeCode_decodeCode m.unpair.2
+      -- conv_rhs => rw [← Nat.bit_decomp n, ← Nat.bit_decomp n.div2]
+      -- simp only [decodeCode.eq_6]
+      -- cases n.bodd <;> cases n.div2.bodd <;> simp [m, encodeCode, IH, IH1, IH2, Nat.bit_val]
+
+
+      unfold c_replace_oracle
+      unfold replace_oracle
+      -- simp [encodeCode_replace_oracle, decodeCode]
+      -- simp [eval_prim]
+
+      cases n.bodd with
+      | false => cases n.div2.bodd with
+        | true =>
+          have h0: (n+4+1)%4=2 := by sorry
+          -- simp only [h0, ↓reduceIte]
+          simp only []
+
+        | false => sorry
+      | true => sorry
+
+
+      -- -- general case
+      -- let m := n.div2.div2
+      -- have hm : m < n + 5 := by
+      --   -- your proof of this inequality
+      --   sorry
+      -- -- continue using `ih m`
+      sorry
+
+@[simp] theorem c_replace_oracle_ev:eval O (c_replace_oracle o) = (replace_oracle o) := by rw [← eval_prim_eq_eval c_replace_oracle_ev_pr]; simp only [c_replace_oracle_evp]
+end Nat.RecursiveIn.Code
+theorem Nat.PrimrecIn.replace_oracle:Nat.PrimrecIn O (replace_oracle o) := by rw [← c_replace_oracle_evp]; apply code_prim_prop c_replace_oracle_ev_pr
+theorem Nat.Primrec.replace_oracle:Nat.Primrec (replace_oracle o) := by exact PrimrecIn.PrimrecIn_Empty PrimrecIn.replace_oracle
+end replace_oracle
+
+
+
+
+
+
+
+
+
+
+
+
+
+
+
+
+
+
+
+
+
+
 
 
 
